Logic/Predicate/FirstOrder/Arith/Basic.lean
@@ -1,0 +1,75 @@
+import Logic.Predicate.FirstOrder.Order.Le
+
+namespace LO
+
+class ORingSymbol (α : Type*) extends
+  Zero α, One α, Add α, Mul α, LT α
+
+attribute [instance] ORingSymbol.mk
+
+namespace ORingSymbol
+
+variable {α : Type*} [ORingSymbol α]
+
+def numeral : ℕ → α
+  | 0     => 0
+  | 1     => 1
+  | n + 2 => numeral (n + 1) + 1
+
+ lemma zero_eq_zero : (Zero.zero : α) = 0 := rfl
+
+ lemma one_eq_one : (One.one : α) = 1 := rfl
+
+end ORingSymbol
+
+@[simp] lemma Nat.numeral_eq : (n : ℕ) → ORingSymbol.numeral n = n
+  | 0     => rfl
+  | 1     => rfl
+  | n + 2 => by simp[ORingSymbol.numeral, Nat.numeral_eq (n + 1)]; rfl
+
+namespace FirstOrder
+
+open Subterm Subformula
+
+class ORing (L : Language) extends
+  Operator.Zero L, Operator.One L, Operator.Add L, Operator.Mul L, Operator.Eq L, Operator.LT L
+
+class Structure.ORing (L : Language) [ORing L]
+    (M : Type w) [Zero M] [One M] [Add M] [Mul M] [LT M] [Structure L M] extends
+  Structure.Zero L M, Structure.One L M, Structure.Add L M, Structure.Mul L M, Structure.Eq L M, Structure.LT L M
+
+attribute [instance] Structure.ORing.mk
+
+namespace Structure
+
+variable [FirstOrder.ORing L] {M : Type u} [ORingSymbol M] [Structure L M] [Structure.ORing L M]
+
+@[simp] lemma numeral_eq_numeral : (z : ℕ) → (Subterm.Operator.numeral L z).val ![] = (ORingSymbol.numeral z : M)
+  | 0     => by simp[ORingSymbol.numeral, Subterm.Operator.numeral_zero]
+  | 1     => by simp[ORingSymbol.numeral, Subterm.Operator.numeral_one]
+  | z + 2 => by simp[ORingSymbol.numeral, Subterm.Operator.numeral_add_two,
+                  Subterm.Operator.val_comp, Matrix.fun_eq_vec₂, numeral_eq_numeral (z + 1)]
+
+end Structure
+
+namespace Arith
+variable [ORing L] {T : Theory L} [EqTheory T] [SubTheory (Theory.Order.Total L) T]
+
+lemma consequence_of (σ : Sentence L)
+  (H : ∀ (M : Type u)
+         [Inhabited M]
+         [ORingSymbol M]
+         [Structure L M]
+         [Structure.ORing L M]
+         [Theory.Mod M T],
+         M ⊧ σ) :
+    T ⊨ σ := consequence_iff_eq.mpr fun M _ _ _ hT =>
+  letI : Theory.Mod (Structure.Model L M) T := ⟨((ElementaryEquiv.modelsTheory (Structure.Model.elementaryEquiv L M)).mp hT)⟩
+  (ElementaryEquiv.models (Structure.Model.elementaryEquiv L M)).mpr
+    (H (Structure.Model L M))
+
+end Arith
+
+end FirstOrder
+
+end LO
